Redesign concurrent/counter to include optional upper bound.

theories/concurrent/counter.v
@@ -3,11 +3,10 @@ From iris.algebra Require Import
 
 From caml5 Require Import
   prelude.
-From caml5.common Require Import
-  tactics.
 From caml5.base_logic Require Import
-  lib.auth_excl
-  lib.auth_nat_max.
+  lib.auth_natinf_max
+  lib.auth_nat_max
+  lib.auth_excl.
 From caml5.lang Require Import
   notations
   proofmode.
@@ -15,15 +14,18 @@ From caml5.concurrent Require Export
   base.
 
 Class CounterG Σ `{!heapGS Σ} := {
-  counter_G_mono_G : AuthNatMaxG Σ ;
+  counter_G_ub_G : AuthNatinfMaxG Σ ;
+  counter_G_lb_G : AuthNatMaxG Σ ;
   counter_G_token_G : inG Σ (authR (gset_disjUR nat)) ;
   counter_G_model_G : AuthExclG Σ natO ;
 }.
-#[local] Existing Instance counter_G_mono_G.
+#[local] Existing Instance counter_G_ub_G.
+#[local] Existing Instance counter_G_lb_G.
 #[local] Existing Instance counter_G_token_G.
 #[local] Existing Instance counter_G_model_G.
 
 Definition counter_Σ := #[
+  auth_natinf_max_Σ ;
   auth_nat_max_Σ ;
   GFunctor (authR (gset_disjUR nat)) ;
   auth_excl_Σ natO
@@ -51,31 +53,44 @@ Section counter_G.
     λ: "t",
       !"t".
 
-  Notation counter_meta_mono :=
-    (nroot .@ "mono").
+  Notation counter_meta_ub :=
+    (nroot .@ "ub").
+  Notation counter_meta_lb :=
+    (nroot .@ "lb").
   Notation counter_meta_token :=
     (nroot .@ "token").
   Notation counter_meta_model :=
     (nroot .@ "model").
 
-  #[local] Definition counter_mono_auth γ_mono dq n :=
-    auth_nat_max_auth γ_mono dq n.
-  #[local] Definition counter_mono_frag γ_mono n :=
-    auth_nat_max_frag γ_mono n.
+  #[local] Definition counter_ub_auth γ_ub ub :=
+    auth_natinf_max_auth γ_ub DfracDiscarded (
+      if ub is Some ub then natinf_nat ub else natinf_inf
+    ).
+  #[local] Definition counter_ub_frag γ_ub n :=
+    auth_natinf_max_frag γ_ub (natinf_nat n).
+
+  #[local] Definition counter_lb_auth γ_lb dq n :=
+    auth_nat_max_auth γ_lb dq n.
+  #[local] Definition counter_lb_frag γ_lb lb :=
+    auth_nat_max_frag γ_lb lb.
   Definition counter_lb t lb : iProp Σ :=
-    ∃ l γ_mono,
+    ∃ l γ_ub γ_lb,
     ⌜t = #l⌝ ∗
-    meta l counter_meta_mono γ_mono ∗
-    counter_mono_frag γ_mono lb.
+    meta l counter_meta_ub γ_ub ∗
+    meta l counter_meta_lb γ_lb ∗
+    counter_ub_frag γ_ub lb ∗
+    counter_lb_frag γ_lb lb.
 
   #[local] Definition counter_token_auth γ_token dq n :=
     own γ_token (●{dq} GSet (set_seq 0 n)).
   #[local] Definition counter_token_frag γ_token n :=
     own γ_token (◯ GSet {[n]}).
   Definition counter_token t n : iProp Σ :=
-    ∃ l γ_token,
+    ∃ l γ_ub γ_token,
     ⌜t = #l⌝ ∗
+    meta l counter_meta_ub γ_ub ∗
     meta l counter_meta_token γ_token ∗
+    counter_ub_frag γ_ub n ∗
     counter_token_frag γ_token n.
 
   #[local] Definition counter_model₁ γ_model n :=
@@ -83,12 +98,14 @@ Section counter_G.
   #[local] Definition counter_model₂ γ_model dq n :=
     auth_excl_auth γ_model dq n.
   Definition counter_model t dq n : iProp Σ :=
-    ∃ l γ_mono γ_token γ_model,
+    ∃ l γ_ub γ_lb γ_token γ_model,
     ⌜t = #l⌝ ∗
-    meta l counter_meta_mono γ_mono ∗
+    meta l counter_meta_ub γ_ub ∗
+    meta l counter_meta_lb γ_lb ∗
     meta l counter_meta_token γ_token ∗
     meta l counter_meta_model γ_model ∗
-    counter_mono_auth γ_mono dq n ∗
+    counter_ub_frag γ_ub n ∗
+    counter_lb_auth γ_lb dq n ∗
     counter_token_auth γ_token dq n ∗
     counter_model₂ γ_model dq n.
 
@@ -96,10 +113,12 @@ Section counter_G.
     ∃ n,
     l ↦ #n ∗
     counter_model₁ γ_model n.
-  Definition counter_inv t ι : iProp Σ :=
-    ∃ l γ_model,
+  Definition counter_inv t ι ub : iProp Σ :=
+    ∃ l γ_ub γ_model,
     ⌜t = #l⌝ ∗
+    meta l counter_meta_ub γ_ub ∗
     meta l counter_meta_model γ_model ∗
+    counter_ub_auth γ_ub ub ∗
     inv ι (counter_inv_inner l γ_model).
 
   #[global] Instance counter_lb_persistent t lb :
@@ -122,8 +141,8 @@ Section counter_G.
   Proof.
     apply _.
   Qed.
-  #[global] Instance counter_inv_persistent t ι :
-    Persistent (counter_inv t ι).
+  #[global] Instance counter_inv_persistent t ι ub :
+    Persistent (counter_inv t ι ub).
   Proof.
     apply _.
   Qed.
@@ -132,16 +151,17 @@ Section counter_G.
     Fractional (λ q, counter_model t (DfracOwn q) n).
   Proof.
     intros q1 q2. iSplit.
-    - iIntros "(%l & %γ_mono & %γ_token & %γ_model & -> & #Hmeta_mono & #Hmeta_token & #Hmeta_model & (Hmono_auth1 & Hmono_auth2) & (Htoken_auth1 & Htoken_auth2) & (Hmodel₂1 & Hmodel₂2))".
-      iSplitL "Hmono_auth1 Htoken_auth1 Hmodel₂1"; repeat iExists _; auto with iFrame.
-    - iIntros "((%_l & %_γ_mono & %_γ_token & %_γ_model & % & #Hmeta_mono & #Hmeta_token & #Hmeta_model & Hmono_auth1 & Htoken_auth1 & Hmodel₂1) & (%l & %γ_mono & %γ_token & %γ_model & % & #_Hmeta_mono & #_Hmeta_token & #_Hmeta_model & Hmono_auth2 & Htoken_auth2 & Hmodel₂2))". simplify.
-      iDestruct (meta_agree with "Hmeta_mono _Hmeta_mono") as %->. iClear "_Hmeta_mono".
+    - iIntros "(%l & %γ_ub & %γ_lb & %γ_token & %γ_model & -> & #Hmeta_ub & #Hmeta_lb & #Hmeta_token & #Hmeta_model & #Hub_frag & (Hlb_auth1 & Hlb_auth2) & (Htoken_auth1 & Htoken_auth2) & (Hmodel₂1 & Hmodel₂2))".
+      iSplitL "Hlb_auth1 Htoken_auth1 Hmodel₂1"; repeat iExists _; iFrame "#∗"; done.
+    - iIntros "((%l & %γ_ub & %γ_lb & %γ_token & %γ_model & -> & #Hmeta_ub & #Hmeta_lb & #Hmeta_token & #Hmeta_model & #Hub_frag & Hlb_auth1 & Htoken_auth1 & Hmodel₂1) & (%_l & %_γ_ub & %_γ_lb & %_γ_token & %_γ_model & %Heq & #_Hmeta_ub & #_Hmeta_lb & #_Hmeta_token & #_Hmeta_model & _ & Hlb_auth2 & Htoken_auth2 & Hmodel₂2))". injection Heq as <-.
+      iDestruct (meta_agree with "Hmeta_ub _Hmeta_ub") as %->. iClear "_Hmeta_ub".
+      iDestruct (meta_agree with "Hmeta_lb _Hmeta_lb") as %->. iClear "_Hmeta_lb".
       iDestruct (meta_agree with "Hmeta_token _Hmeta_token") as %->. iClear "_Hmeta_token".
       iDestruct (meta_agree with "Hmeta_model _Hmeta_model") as %->. iClear "_Hmeta_model".
-      iCombine "Hmono_auth1 Hmono_auth2" as "Hmono_auth".
+      iCombine "Hlb_auth1 Hlb_auth2" as "Hlb_auth".
       iCombine "Htoken_auth1 Htoken_auth2" as "Htoken_auth".
       iCombine "Hmodel₂1 Hmodel₂2" as "Hmodel₂".
-      repeat iExists _. auto with iFrame.
+      repeat iExists _. iFrame "#∗". done.
   Qed.
   #[global] Instance counter_model_as_fractional t q n :
     AsFractional (counter_model t (DfracOwn q) n) (λ q, counter_model t (DfracOwn q) n) q.
@@ -149,71 +169,90 @@ Section counter_G.
     split; [done | apply _].
   Qed.
 
-  Lemma counter_lb_valid t dq n lb :
-    counter_model t dq n -∗
+  Lemma counter_inv_lb_valid t ι ub lb :
+    counter_inv t ι (Some ub) -∗
     counter_lb t lb -∗
-    ⌜lb ≤ n⌝.
+    ⌜lb ≤ ub⌝.
   Proof.
-    iIntros "(%_l & %_γ_mono & %γ_token & %γ_model & % & #Hmeta_mono & #Hmeta_token & #Hmeta_model & Hmono_auth & Htoken_auth & Hmodel₂) (%l & %γ_mono & % & #_Hmeta_mono & Hmono_frag)". simplify.
-    iDestruct (meta_agree with "Hmeta_mono _Hmeta_mono") as %->. iClear "_Hmeta_mono".
-    iApply (auth_nat_max_valid with "Hmono_auth Hmono_frag").
+    iIntros "(%l & %γ_ub & %γ_model & -> & #Hmeta_ub & #Hmeta_model & #Hub_auth & #Hinv) (%_l & %_γ_ub & %_γ_lb & %Heq & #_Hmeta_ub & #_Hmeta_lb & #Hub_frag & #Hlb_frag)". injection Heq as <-.
+    iDestruct (meta_agree with "Hmeta_ub _Hmeta_ub") as %<-. iClear "_Hmeta_ub".
+    iDestruct (auth_natinf_max_valid with "Hub_auth Hub_frag") as %?%(inj natinf_nat). done.
   Qed.
   Lemma counter_lb_le t lb1 lb2 :
     lb2 ≤ lb1 →
     counter_lb t lb1 -∗
     counter_lb t lb2.
   Proof.
-    iIntros "% (%l & %γ_mono & -> & #Hmeta_mono & Hmono_frag)".
-    iDestruct (auth_nat_max_frag_le with "Hmono_frag") as "Hmono_frag"; first done.
+    iIntros "% (%l & %γ_ub & %γ_lb & -> & #Hmeta_ub & #Hmeta_lb & #Hub_frag & Hlb_frag)".
+    iDestruct (auth_natinf_max_frag_le with "Hub_frag") as "#Hub_frag'".
+    { apply natinf_le_proper. done. }
+    iDestruct (auth_nat_max_frag_le with "Hlb_frag") as "Hlb_frag"; first done.
     repeat iExists _. naive_solver.
   Qed.
   Lemma counter_lb_get t dq n :
     counter_model t dq n -∗
     counter_lb t n.
   Proof.
-    iIntros "(%l & %γ_mono & %γ_token & %γ_model & % & #Hmeta_mono & #Hmeta_token & #Hmeta_model & Hmono_auth & Htoken_auth & Hmodel₂)".
-    iDestruct (auth_nat_max_frag_get with "Hmono_auth") as "#Hmono_frag".
+    iIntros "(%l & %γ_ub & %γ_lb & %γ_token & %γ_model & -> & #Hmeta_ub & #Hmeta_lb & #Hmeta_token & #Hmeta_model & #Hub_frag & Hlb_auth & Htoken_auth & Hmodel₂)".
+    iDestruct (auth_nat_max_frag_get with "Hlb_auth") as "#Hlb_frag".
     repeat iExists _. naive_solver.
   Qed.
 
-  Lemma counter_token_valid t dq n m :
-    counter_model t dq n -∗
-    counter_token t m -∗
-    ⌜m < n⌝.
+  Lemma counter_inv_token_ub t ι ub n :
+    counter_inv t ι (Some ub) -∗
+    counter_token t n -∗
+    ⌜n ≤ ub⌝.
   Proof.
-    iIntros "(%_l & %γ_mono & %_γ_token & %γ_model & % & #Hmeta_mono & #Hmeta_token & #Hmeta_model & Hmono_auth & Htoken_auth & Hmodel₂) (%l & %γ_token & % & #_Hmeta_token & Htoken_frag)". simplify.
-    iDestruct (meta_agree with "Hmeta_token _Hmeta_token") as %->. iClear "_Hmeta_token".
-    iDestruct (own_valid_2 with "Htoken_auth Htoken_frag") as %(_ & Hincluded & _)%auth_both_dfrac_valid_discrete.
-    rewrite gset_disj_included -elem_of_subseteq_singleton elem_of_set_seq in Hincluded.
-    naive_solver.
+    iIntros "(%l & %γ_ub & %γ_model & -> & #Hmeta_ub & #Hmeta_model & #Hub_auth & #Hinv) (%_l & %_γ_ub & %_γ_lb & %Heq & #_Hmeta_ub & #_Hmeta_token & #Hub_frag & Htoken_frag)". injection Heq as <-.
+    iDestruct (meta_agree with "Hmeta_ub _Hmeta_ub") as %<-. iClear "_Hmeta_ub".
+    iDestruct (auth_natinf_max_valid with "Hub_auth Hub_frag") as %?%(inj natinf_nat). done.
   Qed.
   Lemma counter_token_exclusive t n :
     counter_token t n -∗
     counter_token t n -∗
     False.
   Proof.
-    iIntros "(%_l & %_γ_token & % & #Hmeta_token & Htoken_frag1) (%l & %γ_token & % & #_Hmeta_token & Htoken_frag2)". simplify.
+    iIntros "(%l & %γ_ub & %γ_token & -> & #Hmeta_ub & #Hmeta_token & #Hub_frag & Htoken_frag1) (%_l & %_γ_ub & %_γ_token & %Heq & #_Hmeta_ub & #_Hmeta_token & _ & Htoken_frag2)". injection Heq as <-.
     iDestruct (meta_agree with "Hmeta_token _Hmeta_token") as %->. iClear "_Hmeta_token".
-    iDestruct (own_valid_2 with "Htoken_frag1 Htoken_frag2") as %?%auth_frag_op_valid%gset_disj_valid_op.
-    set_solver.
+    iDestruct (own_valid_2 with "Htoken_frag1 Htoken_frag2") as %?%auth_frag_op_valid%gset_disj_valid_op. set_solver.
   Qed.
 
-  Lemma counter_model_persist t dq n :
-    counter_model t dq n ==∗
-    counter_model t DfracDiscarded n.
-  Proof.
-    iIntros "(%l & %γ_mono & %γ_token & %γ_model & -> & #Hmeta_mono & #Hmeta_token & #Hmeta_model & Hmono_auth & Htoken_auth & Hmodel₂)".
-    iMod (auth_nat_max_auth_persist with "Hmono_auth") as "Hmono_auth".
-    iMod (own_update with "Htoken_auth") as "Htoken_auth"; first eapply auth_update_auth_persist.
-    iMod (auth_excl_auth_persist with "Hmodel₂") as "Hmodel₂".
-    repeat iExists _. iFrame "∗#". done.
-  Qed.
   Lemma counter_model_valid t dq n :
     counter_model t dq n -∗
     ⌜✓ dq⌝.
   Proof.
-    iIntros "(%l & %γ_mono & %γ_token & %γ_model & -> & #Hmeta_mono & #Hmeta_token & #Hmeta_model & Hmono_auth & Htoken_auth & Hmodel₂)".
+    iIntros "(%l & %γ_ub & %γ_lb & %γ_token & %γ_model & -> & #Hmeta_ub & #Hmeta_lb & #Hmeta_token & #Hmeta_model & #Hub_frag & Hlb_auth & Htoken_auth & Hmodel₂)".
     iApply (auth_excl_auth_valid with "Hmodel₂").
+  Qed.
+  Lemma counter_inv_model_valid t ι ub dq n :
+    counter_inv t ι ub -∗
+    counter_model t dq n -∗
+    ⌜if ub is Some ub then n ≤ ub else True⌝.
+  Proof.
+    iIntros "(%l & %γ_ub & %γ_model & -> & #Hmeta_ub & #Hmeta_model & #Hub_auth & #Hinv) (%_l & %_γ_ub & %γ_lb & %γ_token & %_γ_model & %Heq & #_Hmeta_ub & #Hmeta_lb & #_Hmeta_token & #_Hmeta_model & #Hub_frag & Hlb_auth & Htoken_auth & Hmodel₂)". injection Heq as <-.
+    destruct ub as [ub |]; last done.
+    iDestruct (meta_agree with "Hmeta_ub _Hmeta_ub") as %<-. iClear "_Hmeta_ub".
+    iDestruct (auth_natinf_max_valid with "Hub_auth Hub_frag") as %?%(inj natinf_nat). done.
+  Qed.
+  Lemma counter_model_lb_valid t dq n lb :
+    counter_model t dq n -∗
+    counter_lb t lb -∗
+    ⌜lb ≤ n⌝.
+  Proof.
+    iIntros "(%l & %γ_ub & %γ_lb & %γ_token & %γ_model & -> & #Hmeta_ub & #Hmeta_lb & #Hmeta_token & #Hmeta_model & #Hub_frag & Hlb_auth & Htoken_auth & Hmodel₂) (%_l & %_γ_ub & %_γ_lb & %Heq & #_Hmeta_ub & #_Hmeta_lb & _ & #Hlb_frag)". injection Heq as <-.
+    iDestruct (meta_agree with "Hmeta_lb _Hmeta_lb") as %->. iClear "_Hmeta_lb".
+    iApply (auth_nat_max_valid with "Hlb_auth Hlb_frag").
+  Qed.
+  Lemma counter_model_token_valid t dq n m :
+    counter_model t dq n -∗
+    counter_token t m -∗
+    ⌜m < n⌝.
+  Proof.
+    iIntros "(%l & %γ_ub & %γ_lb & %γ_token & %γ_model & -> & #Hmeta_ub & #Hmeta_lb & #Hmeta_token & #Hmeta_model & #Hub_frag & Hlb_auth & Htoken_auth & Hmodel₂) (%_l & %_γ_ub & %_γ_token & %Heq & #_Hmeta_ub & #_Hmeta_token & _ & Htoken_frag)". injection Heq as <-.
+    iDestruct (meta_agree with "Hmeta_token _Hmeta_token") as %->. iClear "_Hmeta_token".
+    iDestruct (own_valid_2 with "Htoken_auth Htoken_frag") as %(_ & Hincluded & _)%auth_both_dfrac_valid_discrete.
+    rewrite gset_disj_included -elem_of_subseteq_singleton elem_of_set_seq in Hincluded.
+    naive_solver.
   Qed.
   Lemma counter_model_combine t dq1 n1 dq2 n2 :
     counter_model t dq1 n1 -∗
@@ -221,11 +260,11 @@ Section counter_G.
       counter_model t (dq1 ⋅ dq2) n1 ∗
       ⌜n1 = n2⌝.
   Proof.
-    iIntros "(%_l & %_γ_mono & %_γ_token & %_γ_model & % & #Hmeta_mono & #Hmeta_token & #Hmeta_model & Hmono_auth1 & Htoken_auth1 & Hmodel₂1) (%l & %γ_mono & %γ_token & %γ_model & % & #_Hmeta_mono & #_Hmeta_token & #_Hmeta_model & Hmono_auth2 & Htoken_auth2 & Hmodel₂2)". simplify.
-    iDestruct (meta_agree with "Hmeta_mono _Hmeta_mono") as %->. iClear "_Hmeta_mono".
+    iIntros "(%l & %γ_ub & %γ_lb & %γ_token & %γ_model & -> & #Hmeta_ub & #Hmeta_lb & #Hmeta_token & #Hmeta_model & #Hub_frag1 & Hlb_auth1 & Htoken_auth1 & Hmodel₂1) (%_l & %_γ_ub & %_γ_lb & %_γ_token & %_γ_model & %Heq & #_Hmeta_ub & #_Hmeta_lb & #_Hmeta_token & #_Hmeta_model & #Hub_frag2 & Hlb_auth2 & Htoken_auth2 & Hmodel₂2)". injection Heq as <-.
+    iDestruct (meta_agree with "Hmeta_lb _Hmeta_lb") as %->. iClear "_Hmeta_lb".
     iDestruct (meta_agree with "Hmeta_token _Hmeta_token") as %->. iClear "_Hmeta_token".
     iDestruct (meta_agree with "Hmeta_model _Hmeta_model") as %->. iClear "_Hmeta_model".
-    iDestruct (auth_nat_max_auth_combine with "Hmono_auth1 Hmono_auth2") as "(Hmono_auth & <-)".
+    iDestruct (auth_nat_max_auth_combine with "Hlb_auth1 Hlb_auth2") as "(Hlb_auth & <-)".
     iCombine "Htoken_auth1 Htoken_auth2" as "Htoken_auth".
     iDestruct (auth_excl_auth_combine_L with "Hmodel₂1 Hmodel₂2") as "(Hmodel₂ & _)".
     iSplitL; last done. repeat iExists _. iFrame "∗#". done.
@@ -272,42 +311,64 @@ Section counter_G.
     iIntros "Hmodel1 Hmodel2".
     iDestruct (counter_model_ne with "Hmodel1 Hmodel2") as %?; naive_solver.
   Qed.
+  Lemma counter_model_persist t dq n :
+    counter_model t dq n ==∗
+    counter_model t DfracDiscarded n.
+  Proof.
+    iIntros "(%l & %γ_ub & %γ_lb & %γ_token & %γ_model & -> & #Hmeta_ub & #Hmeta_lb & #Hmeta_token & #Hmeta_model & #Hub_frag & Hlb_auth & Htoken_auth & Hmodel₂)".
+    iMod (auth_nat_max_auth_persist with "Hlb_auth") as "Hlb_auth".
+    iMod (own_update with "Htoken_auth") as "Htoken_auth"; first eapply auth_update_auth_persist.
+    iMod (auth_excl_auth_persist with "Hmodel₂") as "Hmodel₂".
+    repeat iExists _. iFrame "∗#". done.
+  Qed.
 
-  Lemma counter_make_spec ι :
+  Lemma counter_make_spec ι ub :
     {{{ True }}}
       counter_make #()
-    {{{ t, RET t; counter_inv t ι ∗ counter_model t (DfracOwn 1) 0 }}}.
+    {{{ t, RET t; counter_inv t ι ub ∗ counter_model t (DfracOwn 1) 0 }}}.
   Proof.
     iIntros "%Φ _ HΦ".
     wp_rec. iApply wp_fupd. wp_apply (wp_alloc with "[//]"). iIntros "%l (Hl & Hmeta)".
-    iMod (auth_nat_max_alloc 0) as "(%γ_mono & Hmono_auth)".
+    iMod (auth_natinf_max_alloc (if ub is Some ub then natinf_nat ub else natinf_inf)) as "(%γ_ub & Hub_auth)".
+    iMod (auth_natinf_max_auth_persist with "Hub_auth") as "Hub_auth".
+    iMod auth_natinf_max_frag_0 as "#Hub_frag".
+    iMod (auth_nat_max_alloc 0) as "(%γ_lb & Hlb_auth)".
     iMod (own_alloc (● GSet ∅)) as "(%γ_token & Htoken_auth)"; first by apply auth_auth_valid.
     iMod (auth_excl_alloc 0) as "(%γ_model & Hmodel₂ & Hmodel₁)"; first done.
-    iDestruct (meta_token_difference _ (↑counter_meta_mono) with "Hmeta") as "(Hmeta_mono & Hmeta)"; first solve_ndisj.
+    iDestruct (meta_token_difference _ (↑counter_meta_ub) with "Hmeta") as "(Hmeta_ub & Hmeta)"; first solve_ndisj.
+    iDestruct (meta_token_difference _ (↑counter_meta_lb) with "Hmeta") as "(Hmeta_lb & Hmeta)"; first solve_ndisj.
     iDestruct (meta_token_difference _ (↑counter_meta_token) with "Hmeta") as "(Hmeta_token & Hmeta)"; first solve_ndisj.
     iDestruct (meta_token_difference _ (↑counter_meta_model) with "Hmeta") as "(Hmeta_model & Hmeta)"; first solve_ndisj.
-    iMod (meta_set _ _ γ_mono with "Hmeta_mono") as "#Hmeta_mono"; first done.
+    iMod (meta_set _ _ γ_ub with "Hmeta_ub") as "#Hmeta_ub"; first done.
+    iMod (meta_set _ _ γ_lb with "Hmeta_lb") as "#Hmeta_lb"; first done.
     iMod (meta_set _ _ γ_token with "Hmeta_token") as "#Hmeta_token"; first done.
     iMod (meta_set _ _ γ_model with "Hmeta_model") as "#Hmeta_model"; first done.
-    iApply "HΦ". iSplitL "Hl Hmodel₁".
-    - iExists l, γ_model. repeat iSplitR; [done.. |].
+    iApply "HΦ". iSplitL "Hub_auth Hl Hmodel₁".
+    - repeat iExists _. iFrame "#∗". iSplitR; first done.
       iApply inv_alloc. iExists 0. iFrame.
-    - iExists l, γ_mono, γ_token, γ_model. iFrame "∗#". done.
+    - repeat iExists _. iFrame "∗#". done.
   Qed.
 
-  Lemma counter_incr_spec t ι :
-    <<< counter_inv t ι | ∀∀ n, counter_model t (DfracOwn 1) n >>>
+  Lemma counter_incr_spec t ι ub :
+    <<<
+      counter_inv t ι ub |
+      ∀∀ n, counter_model t (DfracOwn 1) n ∗ if ub is Some ub then ⌜n < ub⌝ else True
+    >>>
       counter_incr t @ ↑ι
-    <<< counter_model t (DfracOwn 1) (S n) ∗ counter_token t n | RET #n; True >>>.
+    <<<
+      counter_model t (DfracOwn 1) (S n) ∗ counter_token t n |
+      RET #n; True
+    >>>.
   Proof.
-    iIntros "!> %Φ (%l & %γ_model & -> & #Hmeta_model & #Hinv) HΦ".
+    iIntros "!> %Φ (%l & %γ_ub & %γ_model & -> & #Hmeta_ub & #Hmeta_model & #Hub_auth & #Hinv) HΦ".
     wp_rec.
     iInv "Hinv" as "(%n & Hl & Hmodel₁)".
     wp_faa.
-    iMod "HΦ" as "(%_n & (%_l & %γ_mono & %γ_token & %_γ_model & %Heq & #Hmeta_mono & #Hmeta_token & #_Hmeta_model & Hmono_auth & Htoken_auth & Hmodel₂) & _ & HΦ)". injection Heq as <-.
+    iMod "HΦ" as "(%_n & ((%_l & %_γ_ub & %γ_lb & %γ_token & %_γ_model & %Heq & #_Hmeta_ub & #Hmeta_lb & #Hmeta_token & #_Hmeta_model & #Hub_frag & Hlb_auth & Htoken_auth & Hmodel₂) & #Hle) & _ & HΦ)". injection Heq as <-.
+    iDestruct (meta_agree with "Hmeta_ub _Hmeta_ub") as %<-. iClear "_Hmeta_ub".
     iDestruct (meta_agree with "Hmeta_model _Hmeta_model") as %<-. iClear "_Hmeta_model".
     iDestruct (auth_excl_agree_L with "Hmodel₂ Hmodel₁") as %->.
-    iMod (auth_nat_max_update (S n) with "Hmono_auth") as "Hmono_auth"; first lia.
+    iMod (auth_nat_max_update (S n) with "Hlb_auth") as "Hlb_auth"; first lia.
     iMod (own_update _ _ (● GSet (set_seq 0 (S n)) ⋅ ◯ GSet {[n]}) with "Htoken_auth") as "(Htoken_auth & Htoken_frag)".
     { apply auth_update_alloc.
       rewrite set_seq_S_end_union_L. apply gset_disj_alloc_empty_local_update.
@@ -315,37 +376,54 @@ Section counter_G.
     }
     iMod (auth_excl_update' (S n) with "Hmodel₂ Hmodel₁") as "(Hmodel₂ & Hmodel₁)".
     iAssert (counter_token #l n) with "[Htoken_frag]" as "Htoken".
-    { iExists l, γ_token. naive_solver. }
-    iAssert (counter_model #l (DfracOwn 1) (S n)) with "[Hmono_auth Htoken_auth Hmodel₂]" as "Hmodel".
-    { iExists l, γ_mono, γ_token, γ_model. iFrame "∗#". done. }
+    { repeat iExists _. naive_solver. }
+    iAssert (counter_model #l (DfracOwn 1) (S n)) with "[> Hlb_auth Htoken_auth Hmodel₂]" as "Hmodel".
+    { repeat iExists _. iFrame "∗#". iSplitR; first done.
+      iDestruct (auth_natinf_max_frag_get with "Hub_auth") as "Hub_frag'".
+      destruct ub as [ub |].
+      - iDestruct "Hle" as %?.
+        iDestruct (auth_natinf_max_frag_le with "Hub_frag'") as "$"; last done.
+        apply natinf_le_proper. done.
+      - iDestruct (auth_natinf_max_frag_le with "Hub_frag'") as "$"; done.
+    }
     iMod ("HΦ" with "[$Hmodel $Htoken] [//]") as "$".
     iModIntro. iExists (S n). iNext. iFrame.
     assert (n + 1 = S n)%Z as -> by lia. done.
   Qed.
 
-  Lemma counter_get_spec t ι :
-    <<< counter_inv t ι | ∀∀ dq n, counter_model t dq n >>>
+  Lemma counter_get_spec t ι ub :
+    <<<
+      counter_inv t ι ub |
+      ∀∀ dq n, counter_model t dq n
+    >>>
       counter_get t @ ↑ι
-    <<< counter_model t dq n | RET #n; True >>>.
+    <<<
+      counter_model t dq n |
+      RET #n; if ub is Some ub then ⌜n ≤ ub⌝ else True
+    >>>.
   Proof.
-    iIntros "!> %Φ (%l & %γ_model & -> & #Hmeta_model & #Hinv) HΦ".
+    iIntros "!> %Φ (%l & %γ_ub & %γ_model & -> & #Hmeta_ub & #Hmeta_model & #Hub_auth & #Hinv) HΦ".
     wp_rec.
     iInv "Hinv" as "(%n & Hl & Hmodel₁)".
     wp_load.
-    iMod "HΦ" as "(%dq & %_n & (%_l & %γ_mono & %γ_token & %_γ_model & %Heq & #Hmeta_mono & #Hmeta_token & #_Hmeta_model & Hmono_auth & Htoken_auth & Hmodel₂) & _ & HΦ)". injection Heq as <-.
+    iMod "HΦ" as "(%dq & %_n & (%_l & %_γ_ub & %γ_lb & %γ_token & %_γ_model & %Heq & #_Hmeta_ub & #Hmeta_lb & #Hmeta_token & #_Hmeta_model & #Hub_frag & Hlb_auth & Htoken_auth & Hmodel₂) & _ & HΦ)". injection Heq as <-.
+    iDestruct (meta_agree with "Hmeta_ub _Hmeta_ub") as %<-. iClear "_Hmeta_ub".
     iDestruct (meta_agree with "Hmeta_model _Hmeta_model") as %<-. iClear "_Hmeta_model".
     iDestruct (auth_excl_agree_L with "Hmodel₂ Hmodel₁") as %->.
-    iAssert (counter_model #l dq n) with "[Hmono_auth Htoken_auth Hmodel₂]" as "Hmodel".
-    { iExists l, γ_mono, γ_token, γ_model. iFrame "∗#". done. }
-    iMod ("HΦ" with "Hmodel [//]") as "$".
+    iAssert (counter_model #l dq n) with "[Hlb_auth Htoken_auth Hmodel₂]" as "Hmodel".
+    { repeat iExists _. iFrame "∗#". done. }
+    iMod ("HΦ" with "Hmodel []") as "$".
+    { destruct ub as [ub |]; last done.
+      iDestruct (auth_natinf_max_valid with "Hub_auth Hub_frag") as %?%(inj natinf_nat). done.
+    }
     iModIntro. iNext. iExists n. iFrame.
   Qed.
 
-  Lemma counter_unboxed t ι :
-    counter_inv t ι -∗
+  Lemma counter_unboxed t ι ub :
+    counter_inv t ι ub -∗
     ⌜val_is_unboxed t⌝.
   Proof.
-    iIntros "(%l & %γ_model & -> & #Hmeta_model & #Hinv) //".
+    iIntros "(%l & %γ_ub & %γ_model & -> & #Hmeta_ub & #Hmeta_model & #Hub_auth & #Hinv) //".
   Qed.
 End counter_G.
 
